Rehaul bvi_tailrec and add ListAppend support
Previously, bvi_tailrec would perform two very similar phases:
1. Attempting to rewrite function tails with operations occuring in tail
   position.
2. Rewriting the entire function body with the first operation from (1) that
   succeeded.

The rewrite itself performed various things such as changing
associativity of operations and utilizing commutativity when possible.
The process was hard to follow and did not turn out well when ListAppend
(a non-commutative operation) was added to the mix. The procedure has
now been split into a few stages. In addition to being easier to follow,
the optimization can now be made to fail earlier if one of the stages
cannot be performed:

1. Check if function has the right recursion pattern at all, else fail.
2. Attempt to rotate all operations in tail position so that
   applications are right associative.
3. Attempt to move the recursive call to the leftmost position in the
   tree inorder using commutativity (optional).
4. Check if there are any suitable tail positions that can be rewritten
   if the above succeeds.
5. Rewrite the function using the operations from one of these (note
   that at this stage most rewriting has been performed by the earlier
   stages).

compiler/backend/bvi_tailrecScript.sml
@@ -14,43 +14,10 @@ val MEM_exp_size_imp = Q.store_thm ("MEM_exp_size_imp",
 val small_int_def = Define `
   small_int (i:int) <=> -268435457 <= i /\ i <= 268435457`;
 
-val is_arith_op_def = Define `
-  is_arith_op Add       = T ∧
-  is_arith_op Mult      = T ∧
-  is_arith_op Sub       = T ∧
-  is_arith_op Div       = T ∧
-  is_arith_op Mod       = T ∧
-  is_arith_op _         = F
-  `;
-
-val is_list_op_def = Define `
-  is_list_op ListAppend = T /\
-  is_list_op _          = F
-  `;
-
-(* TODO may need some is_list for constructed lists *)
-
-val is_const_def = Define `
-  (is_const (Const i) ⇔ small_int i) ∧
-  (is_const _         ⇔ F)
-  `;
-
-val is_num_rel_def = Define `
-  (is_num_rel LessEq       ⇔ T) ∧
-  (is_num_rel Less         ⇔ T) ∧
-  (is_num_rel Greater      ⇔ T) ∧
-  (is_num_rel GreaterEq    ⇔ T) ∧
-  (is_num_rel (EqualInt _) ⇔ T) ∧
-  (is_num_rel _            ⇔ F)
-  `;
-
 val is_rec_def = Define `
   (is_rec name (bvi$Call _ d _ NONE) ⇔ d = SOME name) ∧
   (is_rec _    _                     ⇔ F)
   `;
-
-val _ = export_rewrites
-  ["is_arith_op_def", "is_list_op_def", "is_const_def", "is_num_rel_def"];
 
 val _ = Datatype `
   assoc_op = Plus
@@ -59,6 +26,11 @@ val _ = Datatype `
            | Noop`;
 
 val _ = Datatype `v_ty = Int | List | Any`;
+
+val op_type_def = Define `
+  op_type Append = List /\
+  op_type Noop   = Any /\
+  op_type _      = Int`;
 
 val to_op_def = Define `
   to_op Plus   = Add        /\
@@ -86,6 +58,13 @@ val op_eq_def = Define `
   (op_eq Times  (Op op xs) <=> op = Mult) /\
   (op_eq Append (Op op xs) <=> op = ListAppend) /\
   (op_eq _      _          <=> F)`;
+
+val op_eq_to_op = Q.store_thm ("op_eq_to_op[simp]",
+  `∀iop op xs.
+      op_eq iop (Op op xs)
+      ⇔
+      op = to_op iop ∧ iop ≠ Noop`,
+  Cases \\ Cases \\ fs [op_eq_def, to_op_def]);
 
 val apply_op_def = Define `
   apply_op op e1 e2 = Op (to_op op) [e1; e2]
@@ -117,12 +96,14 @@ val get_bin_args_def = Define `
 val exp_size_get_bin_args = Q.store_thm ("exp_size_get_bin_args",
   `∀x x1 x2.
      get_bin_args x = SOME (x1, x2) ⇒
-       exp_size x1 < exp_size x ∧
-       exp_size x2 < exp_size x`,
+       exp_size x1 + exp_size x2 < exp_size x`,
   Induct
   \\ rw [get_bin_args_def, exp_size_def]
   \\ every_case_tac
   \\ fs [exp_size_def]);
+
+val opbinargs_def = Define `
+  opbinargs opr exp = if ~op_eq opr exp then NONE else get_bin_args exp`;
 
 val try_update_def = Define `
   (try_update vty NONE     ts = ts) ∧
@@ -131,100 +112,222 @@ val try_update_def = Define `
     then TAKE n ts ++ [vty] ++ DROP (n + 1) ts
     else ts)`;
 
-(* --- Rewriting arithmetic (associative and commutative) --- *)
+(* --- Checking termination guarantees --- *)
 
-val no_err_ar_def = tDefine "no_err_ar" `
-  (no_err_ar ts (Op op xs) ⇔
-    case op of
-      Const i => small_int i ∧ xs = []
-    | Add     => LENGTH xs = 2 ∧ EVERY (no_err_ar ts) xs
-    | Mult    => LENGTH xs = 2 ∧ EVERY (no_err_ar ts) xs
-    | _       => F) ∧
-  (no_err_ar ts (Var i) ⇔ if i < LENGTH ts then EL i ts = Int else F) ∧
-  (no_err_ar ts _       ⇔ F)`
+val term_ok_def = tDefine "term_ok" `
+  (* Variables *)
+  (term_ok ts ty (Var i) <=>
+    if ty = Any then i < LENGTH ts
+    else if i < LENGTH ts then EL i ts = ty
+    else F) /\
+  (* Operations *)
+  (term_ok ts ty (Op op xs) <=>
+    (* List operations *)
+    if (ty = Any \/ ty = List) /\ op = ListAppend then
+      LENGTH xs = 2 /\ EVERY (term_ok ts ty) xs
+    else if (ty = Any \/ ty = List) /\ op = Cons nil_tag then
+      xs = []
+    else if (ty = Any \/ ty = List) /\ op = Cons cons_tag /\ LENGTH xs = 2 then
+      term_ok ts Any (HD xs) /\ term_ok ts List (EL 1 xs)
+    (* Arithmetic *)
+    else if (ty = Any \/ ty = Int) /\ op = Add then
+      LENGTH xs = 2 /\ EVERY (term_ok ts Int) xs
+    else if (ty = Any \/ ty = Int) /\ op = Mult then
+      LENGTH xs = 2 /\ EVERY (term_ok ts Int) xs
+    else if (ty = Any \/ ty = Int) /\ op = Sub then
+      LENGTH xs = 2 /\ EVERY (term_ok ts Int) xs
+    else if (ty = Any \/ ty = Int) /\ ?i. op = Const i /\ small_int i then
+      xs = []
+    (* Other types (accepted as first argument of ::) *)
+    else if ty = Any /\ op = Less then
+      LENGTH xs = 2 /\ EVERY (term_ok ts Int) xs
+    else if ty = Any /\ op = LessEq then
+      LENGTH xs = 2 /\ EVERY (term_ok ts Int) xs
+    else if ty = Any /\ op = Greater then
+      LENGTH xs = 2 /\ EVERY (term_ok ts Int) xs
+    else if ty = Any /\ op = GreaterEq then
+      LENGTH xs = 2 /\ EVERY (term_ok ts Int) xs
+    else F) /\
+  (term_ok ts ty _ <=> F)`
+  (WF_REL_TAC `measure (exp_size o SND o SND)` \\ rw []
+   \\ EVAL_TAC
+   \\ imp_res_tac MEM_exp_size_imp
+   \\ fs [bviTheory.exp_size_def, LENGTH_EQ_NUM_compute]);
+
+(* --- Right-associate all targeted operations --- *)
+
+val rotate_def = tDefine "rotate" `
+  rotate opr exp =
+    case opbinargs opr exp of
+      NONE => exp
+    | SOME (a, c) =>
+        case opbinargs opr a of
+          NONE => exp
+        | SOME (a, b) =>
+            rotate opr (apply_op opr a (apply_op opr b c))`
+  (WF_REL_TAC `measure (\(opr,x).
+    case opbinargs opr x of
+      NONE => exp_size x
+    | SOME (a, c) => exp_size a)`
+  \\ rw [opbinargs_def, apply_op_def, get_bin_args_def]
+  \\ every_case_tac \\ fs [] \\ rw []
+  \\ Cases_on `opr` \\ fs [to_op_def, op_eq_def]
+  \\ fs [bviTheory.exp_size_def]);
+
+val rotate_exp_size = Q.store_thm("rotate_exp_size",
+  `!opr exp. exp_size exp = exp_size (rotate opr exp)`,
+  recInduct (theorem "rotate_ind") \\ rw []
+  \\ rw [opbinargs_def, get_bin_args_def, apply_op_def]
+  \\ once_rewrite_tac [rotate_def]
+  \\ CASE_TAC \\ CASE_TAC \\ fs []
+  \\ CASE_TAC \\ CASE_TAC \\ fs []
+  \\ fs [apply_op_def, opbinargs_def, get_bin_args_def]
+  \\ every_case_tac \\ fs [] \\ rveq
+  \\ Cases_on `opr`
+  \\ fs [to_op_def, bviTheory.exp_size_def, closLangTheory.op_size_def]);
+
+val do_assocr_def = tDefine "do_assocr" `
+  do_assocr opr exp =
+    case opbinargs opr exp of
+      NONE => exp
+    | SOME _ =>
+        case opbinargs opr (rotate opr exp) of
+          NONE => exp
+        | SOME (l, r) =>
+            apply_op opr l (do_assocr opr r)`
   (WF_REL_TAC `measure (exp_size o SND)`
-  \\ Induct \\ rw [bviTheory.exp_size_def] \\ res_tac \\ fs []);
+   \\ rw [opbinargs_def, get_bin_args_def]
+   \\ every_case_tac \\ fs [] \\ rw []
+   \\ qmatch_asmsub_abbrev_tac `rotate _ exp`
+   \\ `exp_size exp = exp_size (rotate opr exp)` by fs [rotate_exp_size]
+   \\ unabbrev_all_tac
+   \\ rfs []
+   \\ fs [bviTheory.exp_size_def])
 
-val is_recl_ar_def = Define `
-  is_recl_ar ts name op exp ⇔
-    is_rec name exp ∨
-    op_eq op exp ∧
-      (case get_bin_args exp of
-        NONE        => F
-      | SOME (x, y) => is_rec name x ∧ no_err_ar ts y)
-  `;
+val assocr_def = Define `
+  (assocr (If x1 x2 x3) = If x1 (assocr x2) (assocr x3)) /\
+  (assocr (Let xs x) = Let xs (assocr x)) /\
+  (assocr (Tick x) = Tick (assocr x)) /\
+  (assocr (Op op xs) =
+    if ~(op = Add \/ op = Mult \/ op = ListAppend) then Op op xs
+    else do_assocr (from_op op) (Op op xs)) /\
+  (assocr exp = exp)`;
 
-val assoc_swap_def = Define `
-  assoc_swap op from into =
-    if ¬op_eq op into then
-      apply_op op into from
-    else
-      case get_bin_args into of
-        NONE        => apply_op op into from
-      | SOME (x, y) => apply_op op x (apply_op op from y)
-  `;
+(* Test do_assocr *)
+val test_tm = ``
+  apply_op Plus
+    (apply_op Plus (Var 0)
+      (apply_op Plus (apply_op Plus (Var 1) (Var 2)) (Var 3)))
+    (apply_op Plus (apply_op Plus (Var 4) (Var 5)) (Var 6))``;
 
-val rewrite_ar_def = tDefine "rewrite_ar" `
-  rewrite_ar ts op loc exp =
-    if ¬op_eq op exp then (F, exp)
-    else
-      case get_bin_args exp of
-        NONE => (F, exp)
-      | SOME (x1, x2) =>
-        let (r1, y1) = rewrite_ar ts op loc x1 in
-        let (r2, y2) = rewrite_ar ts op loc x2 in
-          case (is_recl_ar ts loc op y1, is_recl_ar ts loc op y2) of
-            (T, F) => if no_err_ar ts y2
-                      then (T, assoc_swap op y2 y1) else (F, exp)
-          | (F, T) => if no_err_ar ts y1
-                      then (T, assoc_swap op y1 y2) else (F, exp)
-          | _      => (F, exp)
-  `
-  (WF_REL_TAC `measure (exp_size o SND o SND o SND)`
-  \\ rw [exp_size_get_bin_args]);
+val succ_tm = ``
+  apply_op Plus (Var 0) (apply_op Plus (Var 1) (apply_op Plus (Var 2)
+    (apply_op Plus (Var 3)
+    (apply_op Plus (Var 4) (apply_op Plus (Var 5) (Var 6))))))``;
 
-(* --- Rewriting append (only associative) --- *)
+val do_assocr_test = Q.store_thm ("do_assocr_test",
+  `do_assocr Plus ^test_tm = ^succ_tm`, EVAL_TAC);
 
-(* TODO *)
-val no_err_app = Define `
-  (no_err_app ts (Op op xs) <=> op = ListAppend) /\
-  (no_err_app ts _          <=> F)
-  `;
+(* --- Do commutative shifts of recursive calls --- *)
 
-val is_recl_app_def = Define `
-  is_recl_app ts name op exp <=>
-    is_rec name exp \/
-    op_eq op exp /\
-      (case get_bin_args exp of
-         NONE => F
-       | SOME (x, y) => is_rec name x /\ no_err_app ts y)
-  `;
+(* Assumes that tree is rotated right *)
+val do_comml_def = tDefine "do_comml" `
+  do_comml loc opr exp =
+    case opbinargs opr exp of
+      NONE => exp
+    | SOME (l, r) =>
+        if is_rec loc r then apply_op opr r l
+        else if is_rec loc l then exp else
+          case opbinargs opr (do_comml loc opr r) of
+            NONE => exp
+          | SOME (r1, r2) =>
+              if is_rec loc r2 then
+                apply_op opr r2 (apply_op opr l r1)
+              else if is_rec loc r1 then
+                apply_op opr r1 (apply_op opr l r2)
+              else exp`
+  (WF_REL_TAC `measure (exp_size o SND o SND)`
+  \\ rw [opbinargs_def]
+  \\ imp_res_tac exp_size_get_bin_args \\ fs []);
 
-val rewrite_app_def = tDefine "rewrite_app" `
-  rewrite_app ts op loc exp =
-    if ~op_eq op exp then (F, exp) else
-      case get_bin_args exp of
-        NONE => (F, exp)
-      | SOME (x1, x2) =>
-          let (r1, y1) = rewrite_app ts op loc x1 in
-          let (r2, y2) = rewrite_app ts op loc x2 in
-            if ~is_recl_app ts loc op y1 then (F, exp)
-            else if ~no_err_app ts y2    then (F, exp)
-            else (T, assoc_swap op y2 y1)`
-  (WF_REL_TAC `measure (exp_size o SND o SND o SND)`
-   \\ rw [exp_size_get_bin_args]) ;
+val comml_def = Define `
+  (comml loc (If x1 x2 x3) = If x1 (comml loc x2) (comml loc x3)) /\
+  (comml loc (Let xs x) = Let xs (comml loc x)) /\
+  (comml loc (Tick x) = Tick (comml loc x)) /\
+  (comml loc (Op op xs) =
+    if ~(op = Add \/ op = Mult) then Op op xs
+    else do_comml loc (from_op op) (Op op xs)) /\
+  (comml loc exp = exp)`;
 
-(* --- Pre-rewrite analysis (correct types and tail positions) --- *)
+(* Test do_comml *)
+
+val test_tm = ``
+  apply_op Plus (Var 0) (apply_op Plus (Call 0 (SOME 0) [] NONE) (Var 1))``;
+
+val succ_tm = ``
+  apply_op Plus (Call 0 (SOME 0) [] NONE) (apply_op Plus (Var 0) (Var 1))``;
+
+val do_comml_test1 = Q.store_thm("do_comml_test1",
+  `do_comml 0 Plus ^test_tm = ^succ_tm`, EVAL_TAC);
+
+val test_tm = ``apply_op Times (Var 0) (Call 0 (SOME 0) [] NONE)``
+val succ_tm = ``apply_op Times (Call 0 (SOME 0) [] NONE) (Var 0)``;
+val do_comml_test2 = Q.store_thm("do_comml_test2",
+  `do_comml 0 Times ^test_tm = ^succ_tm`, EVAL_TAC);
+
+(* --- Simple tail checking before rewriting --- *)
+
+(* Check if ok to lift xs into accumulator *)
+val check_op_def = Define `
+  check_op ts opr loc exp =
+    case opbinargs opr exp of
+      NONE => F
+    | SOME (f, xs) => is_rec loc f /\ term_ok ts (op_type opr) xs`;
+
+(* --- Type analysis --- *)
 
 val decide_ty_def = Define `
   (decide_ty Int  Int  = Int)  /\
   (decide_ty List List = List) /\
   (decide_ty _    _    = Any)`;
 
+val _ = export_rewrites ["decide_ty_def"]
+
 val LAST1_def = Define `
   LAST1 []      = NONE   /\
   LAST1 [x]     = SOME x /\
   LAST1 (x::xs) = LAST1 xs`;
+
+val update_context_def = Define `
+  update_context ty ts x1 x2 =
+    MAP2 (\a b. if a = ty \/ b = ty then ty else Any)
+      (try_update ty (index_of x1) ts)
+      (try_update ty (index_of x2) ts)
+  `;
+
+val arg_ty_def = Define `
+  arg_ty Add        = Int /\
+  arg_ty Sub        = Int /\
+  arg_ty Mult       = Int /\
+  arg_ty Div        = Int /\
+  arg_ty Mod        = Int /\
+  arg_ty LessEq     = Int /\
+  arg_ty Less       = Int /\
+  arg_ty Greater    = Int /\
+  arg_ty GreaterEq  = Int /\
+  arg_ty ListAppend = List /\
+  arg_ty _          = Any`;
+
+val op_ty_def = Define `
+  (op_ty Add        = Int) /\
+  (op_ty Sub        = Int) /\
+  (op_ty Mult       = Int) /\
+  (op_ty Div        = Int) /\
+  (op_ty Mod        = Int) /\
+  (op_ty ListAppend = List) /\
+  (op_ty (Cons tag) = if tag = nil_tag \/ tag = cons_tag then List else Any) /\
+  (op_ty (Const i)  = if small_int i then Int else Any) /\
+  (op_ty _          = Any)`;
 
 (* Gather information about expressions:
 
@@ -235,8 +338,6 @@ val LAST1_def = Define `
        context.
      - Check if tail positions carry suitable operation (Add/Mult) and track
        branch of origin for the operation in conditionals.
-
-  TODO Add case for ListAppend
 *)
 val scan_expr_def = tDefine "scan_expr" `
   (scan_expr ts loc [] = []) ∧
@@ -250,10 +351,8 @@ val scan_expr_def = tDefine "scan_expr" `
     let (ti, tyi, _, oi) = HD (scan_expr ts loc [xi]) in
     let (tt, ty1, _, ot) = HD (scan_expr ti loc [xt]) in
     let (te, ty2, _, oe) = HD (scan_expr ti loc [xe]) in
-      [(MAP2 decide_ty tt te, decide_ty ty1 ty2, IS_SOME oe,
-        case ot of
-          NONE => oe
-        | _    => ot)]) ∧
+    let op = case ot of NONE => oe | _ => ot in
+      [(MAP2 decide_ty tt te, decide_ty ty1 ty2, IS_SOME oe, op)]) ∧
   (scan_expr ts loc [Let xs x] =
     let ys = scan_expr ts loc xs in
     let tt = MAP (FST o SND) ys in
@@ -264,26 +363,13 @@ val scan_expr_def = tDefine "scan_expr" `
   (scan_expr ts loc [Tick x] = scan_expr ts loc [x]) ∧
   (scan_expr ts loc [Call t d xs h] = [(ts, Any, F, NONE)]) ∧
   (scan_expr ts loc [Op op xs] =
-    let ok_type = (is_arith_op op ∨ is_const op) in
-    let iop =
-      if op = Add ∨ op = Mult then
-        let iop = from_op op in
-          if (FST (rewrite_ar ts iop loc (Op op xs)))
-          then SOME iop
-          else NONE
-      else
-        NONE
-      in
-    let tt =
-      if ¬(is_arith_op op ∨ is_num_rel op) then ts
-      else
-        case get_bin_args (Op op xs) of
-          NONE        => ts
-        | SOME (x, y) =>
-            MAP2 (λa b. if a = Int ∨ b = Int then Int else Any)
-              (try_update Int (index_of x) ts)
-              (try_update Int (index_of y) ts)
-    in [(tt, if ok_type then Int else Any, F, iop)])`
+    let opr = from_op op in
+    let iop = if check_op ts opr loc (Op op xs) then SOME opr else NONE in
+    let tt  =
+      case get_bin_args (Op op xs) of
+        NONE => ts
+      | SOME (x, y) => update_context (arg_ty op) ts x y
+    in [(tt, op_ty op, F, iop)])`
     (WF_REL_TAC `measure (exp2_size o SND o SND)`);
 
 val push_call_def = Define `
@@ -292,51 +378,59 @@ val push_call_def = Define `
   (push_call _ _ _ _ _ = dummy)
   `;
 
-val mk_tailcall_def = Define `
-  mk_tailcall ts n op name acc exp =
-    case rewrite_ar ts op name exp of
-      (F, exp2) => apply_op op exp2 (Var acc)
-    | (T, exp2) =>
-        (case get_bin_args exp2 of
-          NONE => dummy
-        | SOME (call, exp3) =>
-          push_call n op acc exp3 (args_from call))
-  `;
-
-(* TODO Add case for ListAppend *)
 val rewrite_def = Define `
-  (rewrite (loc, next, op, acc, ts) (Var n) = (F, Var n)) ∧
-  (rewrite (loc, next, op, acc, ts) (If xi xt xe) =
-    let (ti, tyi, ri, iop) = HD (scan_expr ts loc [xi]) in
-    let (rt, yt) = rewrite (loc, next, op, acc, ti) xt in
-    let (re, ye) = rewrite (loc, next, op, acc, ti) xe in
-    let zt = if rt then yt else apply_op op xt (Var acc) in
-    let ze = if re then ye else apply_op op xe (Var acc) in
-      (rt ∨ re, If xi zt ze)) ∧
-  (rewrite (loc, next, op, acc, ts) (Let xs x) =
+  (rewrite loc next opr acc ts (Var n) = (F, Var n)) /\
+  (rewrite loc next opr acc ts (If x1 x2 x3) =
+    let t1 = FST (HD (scan_expr ts loc [x1])) in
+    let (r2, y2) = rewrite loc next opr acc t1 x2 in
+    let (r3, y3) = rewrite loc next opr acc t1 x3 in
+    let z2 = if r2 then y2 else apply_op opr x2 (Var acc) in
+    let z3 = if r3 then y3 else apply_op opr x3 (Var acc) in
+      (r2 \/ r3, If x1 z2 z3)) /\
+  (rewrite loc next opr acc ts (Let xs x) =
     let ys = scan_expr ts loc xs in
     let tt = MAP (FST o SND) ys in
-    let tr = (case LAST1 ys of SOME c => FST c | NONE => ts) in
-    let (r, y) = rewrite (loc, next, op, acc + LENGTH xs, tt ++ tr) x in
-      (r, Let xs y)) ∧
-  (rewrite (loc, next, op, acc, ts) (Tick x) =
-    let (r, y) = rewrite (loc, next, op, acc, ts) x in (r, Tick y)) ∧
-  (rewrite (loc, next, op, acc, ts) (Raise x) = (F, Raise x)) ∧
-  (rewrite (loc, next, op, acc, ts) exp =
-    case rewrite_ar ts op loc exp of
-      (F, _)    => (F, apply_op op exp (Var acc))
-    | (T, exp1) =>
-      case get_bin_args exp1 of
-        NONE              => (F, apply_op op exp (Var acc))
-      | SOME (call, exp2) => (T, push_call next op acc exp2 (args_from call)))`;
+    let tr = case LAST1 ys of NONE => ts | SOME c => FST c in
+    let (r, y) = rewrite loc next opr (acc + LENGTH xs) (tt ++ tr) x in
+      (r, Let xs y)) /\
+  (rewrite loc next opr acc ts (Tick x) =
+    let (r, y) = rewrite loc next opr acc ts x in
+      (r, Tick y)) /\
+  (rewrite loc next opr acc ts exp =
+    if ~check_op ts opr loc exp then (F, exp) else
+      case opbinargs opr exp of
+        NONE => (F, exp)
+      | SOME (f, xs) => (T, push_call next opr acc xs (args_from f)))`
 
-(* TODO ty <> Int ==> NONE ~> ty = Any ==> NONE *)
+(* --- Top-level expression check --- *)
+
+val has_rec_def = tDefine "has_rec" `
+  (has_rec loc (If x1 x2 x3) <=> has_rec loc x2 \/ has_rec loc x3) /\
+  (has_rec loc (Let xs x) <=> has_rec loc x) /\
+  (has_rec loc (Tick x) <=> has_rec loc x) /\
+  (has_rec loc (Op op xs) <=> EXISTS (is_rec loc) xs \/ EXISTS (has_rec loc) xs) /\
+  (has_rec loc _ <=> F)`
+  (WF_REL_TAC `measure (exp_size o SND)` \\ rw []
+   \\ imp_res_tac MEM_exp_size_imp \\ fs []);
+
+val test1_tm = ``Let [] (Call 0 (SOME 0) [] NONE)``
+val has_rec_test1 = Q.store_thm("has_rec_test1",
+  `has_rec 0 ^test1_tm <=> F`, EVAL_TAC);
+
+val test2_tm = ``Op Add [Call 0 (SOME 0) [] NONE; Var 0]``
+val has_rec_test2 = Q.store_thm("has_rec_test2",
+  `has_rec 0 ^test2_tm <=> T`, EVAL_TAC);
+
 val check_exp_def = Define `
   check_exp loc arity exp =
-    case scan_expr (REPLICATE arity Any) loc [exp] of
-      [] => NONE
-    | (ts,ty,r,op)::_ =>
-      if ty ≠ Int then NONE else op`;
+    if ~has_rec loc exp then NONE else
+      let expa = assocr exp in
+      let expc = comml loc expa in
+      let context = REPLICATE arity Any in
+        case scan_expr context loc [expc] of
+          [] => NONE
+        | (ts,ty,r,op)::_ =>
+          if ty = Any then NONE else op`;
 
 val let_wrap_def = Define `
   let_wrap arity id exp =
@@ -351,8 +445,10 @@ val compile_exp_def = Define `
     case check_exp loc arity exp of
       NONE    => NONE
     | SOME op =>
-      let ts       = REPLICATE arity Any in
-      let (r, opt) = rewrite (loc, next, op, arity, ts) exp in
+      let context  = REPLICATE arity Any in
+      let expa = assocr exp in
+      let expc = comml loc expa in
+      let (r, opt) = rewrite loc next op arity context expc in
       let aux      = let_wrap arity (id_from_op op) opt in
         SOME (aux, opt)`;
 
@@ -391,10 +487,37 @@ val scan_expr_HD_SING = Q.store_thm ("scan_expr_HD_SING[simp]",
 val check_exp_SOME_simp = Q.store_thm ("check_exp_SOME_simp[simp]",
   `check_exp loc arity exp = SOME op <=>
      ?ts ty r.
-       scan_expr (REPLICATE arity Any) loc [exp] = [(ts,Int,r,SOME op)]`,
+       has_rec loc exp /\
+       scan_expr (REPLICATE arity Any) loc [comml loc (assocr exp)] = [(ts,ty,r,SOME op)] /\
+       ty <> Any`,
   simp [check_exp_def]
-  \\ `LENGTH (scan_expr (REPLICATE arity Any) loc [exp]) = LENGTH [exp]` by fs []
+  \\ `LENGTH (scan_expr (REPLICATE arity Any) loc [comml loc (assocr exp)]) = LENGTH [exp]` by fs []
   \\ EVERY_CASE_TAC \\ fs []);
+
+(* --- Test rewriting --- *)
+
+val fac_tm = ``
+  Let [Op LessEq [Var 0; Op (Const 1) []]]
+    (If (Var 0)
+       (Op (Const 1) [])
+       (Let [Op Sub [Var 1; Op (Const 1) []]]
+         (Op Mult [Var 2; Call 0 (SOME 0) [Var 0] NONE])))``
+
+val opt_tm = ``
+  Let [Op LessEq [Var 0; Op (Const 1) []]]
+     (If (Var 0) (Op Mult [Op (Const 1) []; Var 2])
+        (Let [Op Sub [Var 1; Op (Const 1) []]]
+           (Call 0 (SOME 1) [Var 0; Op Mult [Var 2; Var 3]]
+              NONE)))``
+val aux_tm = ``Let [Var 0; Op (Const 1) []] ^opt_tm``
+
+
+val fac_check_exp = Q.store_thm("fac_check_exp",
+  `check_exp 0 1 ^fac_tm = SOME Times`,
+  EVAL_TAC);
+
+val fac_compile_exp = Q.store_thm("fac_compile_exp",
+  `compile_exp 0 1 1 ^fac_tm = SOME (^aux_tm, ^opt_tm)`, EVAL_TAC);
 
 val _ = export_theory();
 
